pi transition

thys/Pi_Calculus/Pi_Transition.thy
@@ -1,5 +1,8 @@
 (* Here we instantiate the general enhanced rule induction to 
-the (todo: lazy/eager) pi-calculus transition system
+the "early" pi-calculus transition system.
+the adjective refers to the fact that inputs are instantiated 
+at transition time (whereas a "late" semantics would 
+have transitons with bound inputs)
  *)
 theory Pi_Transition
 imports Commitment 
@@ -12,40 +15,86 @@ begin
 print_locales
 interpretation Small where dummy = "undefined :: var" 
 apply standard
-by (simp_all add: infinite_var regularCard_var)  
+by (simp_all add: infinite_var regularCard_var)
+
+datatype (vars:'a) action = finp 'a 'a | fout 'a 'a | bout 'a 'a | tau 
+
+type_synonym act = "var action"
+
+fun Cmt :: "act \<Rightarrow> trm \<Rightarrow> cmt" where 
+ "Cmt (finp x y) P = Finp x y P"
+|"Cmt (fout x y) P = Fout x y P"
+|"Cmt (bout x y) P = Bout x y P"
+|"Cmt tau P = Tau P"
+
+fun bvars :: "act \<Rightarrow> var list" where 
+ "bvars (bout x y) = [y]"
+|"bvars _ = []" 
+
+abbreviation "swapa act x y \<equiv> map_action (id(x:=y,y:=x)) act"
  
 
-(* AN EXAMPLE INDUCTIVE DEFINITION *)
-(* (a reduced form of) small trans semantics *) 
+(* The "late" transition relation  *)
 inductive trans :: "trm \<Rightarrow> cmt \<Rightarrow> bool" where
 Inp: "x \<notin> {a,u} \<Longrightarrow> trans (Inp a x P) (Finp a u (usub P u x))"
-|
+(* |
 Out: "trans (Out a x P) (Fout a x P)"
 |
 Tau: "trans P (Tau P)"
+|
+Match: "trans P C \<Longrightarrow> trans (Match a a P) C"
+|
+Sum1: "trans P1 C \<Longrightarrow> trans (Sum P1 P2) C"
+|
+Sum2: "trans P2 C \<Longrightarrow> trans (Sum P1 P2) C"
+*)
+|
+Open: "trans P (Fout a x P') \<Longrightarrow> a \<noteq> x \<Longrightarrow> 
+       trans (Res x P) (Bout a x P')"
+|
+ScopeF: "trans P (Cmt act P') \<Longrightarrow> y \<notin> vars act \<Longrightarrow> 
+   trans (Res y P) (Cmt act (Res y P'))"
+|
+ScopeB: "trans P (Bout a x P') \<Longrightarrow> y \<notin> {a,x} \<union> FFVars P \<Longrightarrow> x \<noteq> a
+   \<Longrightarrow> 
+   trans (Res y P) (Bout a x (Res y P'))"
+|
+Par1: "trans P1 (Cmt act P1') \<Longrightarrow> set (bvars act) \<inter> FFVars P2 = {} \<Longrightarrow> 
+   trans (Par P1 P2) (Cmt act (Par P1' P2))" 
+(* |
+Par2: "trans P2 (Cmt act P2') \<Longrightarrow> bvars act \<inter> FFVars P1 = {} \<Longrightarrow> 
+   trans (Par P1 P2) (Cmt act (Par P1 P2'))" *)
+|
+Com1: "trans P1 (Finp a x P1') \<Longrightarrow> trans P2 (Fout a x P2') \<Longrightarrow> 
+   trans (Par P1 P2) (Tau (Par P1' P2'))" 
+(* |
+Com2: "trans P1 (Fout a x P1') \<Longrightarrow> trans P2 (Finp a x P2') \<Longrightarrow> 
+   trans (Par P1 P2) (Tau (Par P1' P2'))"  *)
+|
+Close1: "trans P1 (Finp a x P1') \<Longrightarrow> trans P2 (Bout a x P2') \<Longrightarrow> 
+   x \<notin> {a} \<union> FFVars P1 \<union> FFVars P2 \<Longrightarrow>
+   trans (Par P1 P2) (Bout a x (Par P1' P2'))" 
+(* |
+Close2: "trans P1 (Bout a x P1') \<Longrightarrow> trans P2 (Finp a x P2') \<Longrightarrow> 
+   x \<notin> {a} \<union> FFVars P1 \<union> FFVars P2 \<Longrightarrow>
+   trans (Par P1 P2) (Bout a x (Par P1' P2'))" 
+|
+Bang: "trans (Par P (Bang P)) C \<Longrightarrow> trans (Bang P) C"
+*)
 
 
-
-
-term 
-| App: "trans e1 e1' \<Longrightarrow> trans e2 e2' \<Longrightarrow> trans (App e1 e2) (App e1' e2')"
-| Xi: "trans e e' \<Longrightarrow> trans (Abs x e) (Abs x e')"
-| PBeta: "trans e1 e1' \<Longrightarrow> trans e2 e2' \<Longrightarrow> trans (App (Abs x e1) e2) (tvsubst (Var(x:=e2')) e1')"
-
-thm trans_def
 
 (* INSTANTIATING THE Components LOCALE: *)
 
-type_synonym T = "trm \<times> trm"
-type_synonym V = "var list" (* in this case, could have also taken to be 'a option; 
-and the most uniform approach would have been 'a + unit + 'a + 'a *)
+type_synonym T = "trm \<times> cmt"
+type_synonym V = "var list" 
 
 
 definition Tmap :: "(var \<Rightarrow> var) \<Rightarrow> T \<Rightarrow> T" where 
-"Tmap f \<equiv> map_prod (rrename_term f) (rrename_term f)"
+"Tmap f \<equiv> map_prod (rrename f) (rrename_commit f)"
 
 fun Tfvars :: "T \<Rightarrow> var set" where 
-"Tfvars (e1,e2) = FFVars_term e1 \<union> FFVars_term e2"
+"Tfvars (e1,e2) = FFVars e1 \<union> FFVars_commit e2"
 
 definition Vmap :: "(var \<Rightarrow> var) \<Rightarrow> V \<Rightarrow> V" where 
 "Vmap \<equiv> map"
@@ -53,67 +102,224 @@ definition Vmap :: "(var \<Rightarrow> var) \<Rightarrow> V \<Rightarrow> V" whe
 fun Vfvars :: "V \<Rightarrow> var set" where 
 "Vfvars v = set v"
 
+lemmas commit_internal.FFVars_rrenames[simp]
+
 interpretation Components where dummy = "undefined :: var" and 
 Tmap = Tmap and Tfvars = Tfvars
 and Vmap = Vmap and Vfvars = Vfvars 
 apply standard unfolding ssbij_def Tmap_def Vmap_def
   using small_Un small_def term.card_of_FFVars_bounds
-  apply (auto simp: term.rrename_id0s map_prod.comp term.rrename_comp0s inf_A)  
-  by auto 
+    commit_internal.card_of_FFVars_bounds(2)
+  apply (auto simp: term.rrename_id0s map_prod.comp term.rrename_comp0s 
+        commit_internal.rrename_cong_ids(2)
+        commit_internal.rrename_id0s commit_internal.rrename_comp0s(2)
+          inf_A) 
+  by blast 
 
 definition G :: "(T \<Rightarrow> bool) \<Rightarrow> V \<Rightarrow> T \<Rightarrow> bool"
 where
 "G \<equiv> \<lambda>R v t.  
-         (v = [] \<and> fst t = snd t)
-         \<or>
-         (\<exists>e1 e1' e2 e2'. v = [] \<and> fst t = App e1 e2 \<and> snd t = App e1' e2' \<and> 
-                           R (e1,e1') \<and> R (e2,e2')) 
-         \<or>
-         (\<exists>x e e'. v = [x] \<and> fst t = Abs x e \<and> snd t = Abs x e' \<and> R (e,e'))
-         \<or>
-         (\<exists>x e1 e1' e2 e2'. v = [x] \<and> fst t = App (Abs x e1) e2 \<and> snd t = tvsubst (Var(x := e2')) e1' \<and> 
-            R (e1,e1') \<and> R (e2,e2'))"
+ (\<exists>x a u P. 
+    v = [x] \<and> fst t = Inp a x P \<and> snd t = Finp a u (usub P u x) \<and> 
+    x \<notin> {a,u})
+ \<or> 
+ (\<exists>P a x P'. 
+    v = [x] \<and> fst t = Res x P \<and> snd t = Bout a x P' \<and> 
+    a \<noteq> x \<and> 
+    R (P,Fout a x P')) 
+ \<or>
+ (\<exists> P act P' y. 
+    v = bvars act @ [y] \<and> fst t = Res y P \<and> snd t = Cmt act (Res y P') \<and>  
+    y \<notin> vars act \<and> 
+    R (P, Cmt act P'))
+ \<or>
+ (\<exists> P a x P' y. 
+    v = [y,x] \<and> fst t = Res y P \<and> snd t = Bout a x (Res y P') \<and>  
+    y \<notin> {a,x} \<union> FFVars P \<and> x \<noteq> a \<and>  
+    R (Res y P, Bout a x (Res y P')))
+ \<or>
+ (\<exists>P1 act P1' P2. 
+    v = bvars act \<and> fst t = Par P1 P2 \<and> snd t = Cmt act (Par P1' P2) \<and> 
+    set (bvars act) \<inter> FFVars P2 = {} \<and> 
+    R (P1, Cmt act P1'))
+ \<or>
+ (\<exists>P1 a x P1' P2 P2'. 
+    v = [] \<and> fst t = Par P1 P2 \<and> snd t = Tau (Par P1' P2') \<and>  
+    R (P1, Finp a x P1') \<and> R (P2, Fout a x P2'))
+ \<or>
+ (\<exists>P1 a x P1' P2 P2'. 
+    v = [] \<and> fst t = Par P1 P2 \<and> snd t = Bout a x (Par P1' P2') \<and>  
+    x \<notin> {a} \<union> FFVars P1 \<union> FFVars P2 \<and> 
+    R (P1, Finp a x P1') \<and> R (P2, Bout a x P2'))
+"
 
 
 (* VERIFYING THE HYPOTHESES FOR BARENDREGT-ENHANCED INDUCTION: *)
 
 lemma GG_mono: "R \<le> R' \<Longrightarrow> G R v t \<Longrightarrow> G R' v t"
-unfolding G_def by fastforce
+unfolding G_def by (smt (z3) le_boolE le_funD)
+
+thm term.rrename_comps
+
+find_theorems rrename_commit Finp
+
+
+lemma rrename_commit_Finp[simp]: "bij \<sigma> \<and> |supp \<sigma>| <o |UNIV::var set| \<Longrightarrow> 
+  rrename_commit \<sigma> (Finp a u P) = Finp (\<sigma> a) (\<sigma> u) (rrename \<sigma> P)"
+sorry
+
+lemma rrename_commit_Fout[simp]: "bij \<sigma> \<and> |supp \<sigma>| <o |UNIV::var set| \<Longrightarrow> 
+  rrename_commit \<sigma> (Fout a u P) = Fout (\<sigma> a) (\<sigma> u) (rrename \<sigma> P)"
+sorry
+
+lemma rrename_commit_Bout[simp]: "bij \<sigma> \<and> |supp \<sigma>| <o |UNIV::var set| \<Longrightarrow> 
+  rrename_commit \<sigma> (Bout a u P) = Bout (\<sigma> a) (\<sigma> u) (rrename \<sigma> P)"
+sorry
+
+lemma rrename_commit_Tau[simp]: "bij \<sigma> \<and> |supp \<sigma>| <o |UNIV::var set| \<Longrightarrow> 
+  rrename_commit \<sigma> (Tau P) = Tau (rrename \<sigma> P)"
+sorry
+
+
+lemma rrename_usub[simp]: "bij \<sigma> \<and> |supp \<sigma>| <o |UNIV::var set| \<Longrightarrow>  
+ rrename \<sigma> (usub P u x) = usub (rrename \<sigma> P) (\<sigma> u) (\<sigma> x)"
+sorry
+
+lemma bvars_map_action[simp]: "bvars (map_action \<sigma> act) = map \<sigma> (bvars act)"
+by (cases act, auto)
+
+lemma rrename_commit_Cmt[simp]: 
+"bij \<sigma> \<and> |supp \<sigma>| <o |UNIV::var set| \<Longrightarrow>  
+ rrename_commit \<sigma> (Cmt act P) = Cmt (map_action \<sigma> act) (rrename \<sigma> P)"
+by (cases act, auto)
+
+lemmas action.set_map[simp]
+
+(* lemma FFVars_commit_Cmt[simp]: "FFVars_commit (Cmt act P) = FFVars P" *)
+ 
 
 (* NB: Everything is passed \<sigma>-renamed as witnesses to exI *)
 lemma GG_equiv: "ssbij \<sigma> \<Longrightarrow> G R v t \<Longrightarrow> G (\<lambda>t'. R (Tmap (inv \<sigma>) t')) (Vmap \<sigma> v) (Tmap \<sigma> t)"
 unfolding G_def apply(elim disjE)
+  (* *)
   subgoal apply(rule disjI1)
-  subgoal  
+  subgoal apply(elim exE) subgoal for x a u P
+  apply(rule exI[of _ "\<sigma> x"]) apply(rule exI[of _ "\<sigma> a"]) 
+  apply(rule exI[of _ "\<sigma> u"]) apply(rule exI[of _ "rrename \<sigma> P"])
   apply(cases t) unfolding ssbij_def small_def Tmap_def Vmap_def 
-  by simp . 
+  by (simp add: term.rrename_comps) . . 
   (* *)
   subgoal apply(rule disjI2, rule disjI1)
-  subgoal apply(elim exE) subgoal for e1 e1' e2 e2'
-  apply(rule exI[of _ "rrename_term \<sigma> e1"]) apply(rule exI[of _ "rrename_term \<sigma> e1'"]) 
-  apply(rule exI[of _ "rrename_term \<sigma> e2"]) apply(rule exI[of _ "rrename_term \<sigma> e2'"])
+  subgoal apply(elim exE) subgoal for P a x P'
+  apply(rule exI[of _ "rrename \<sigma> P"])
+  apply(rule exI[of _ "\<sigma> a"]) apply(rule exI[of _ "\<sigma> x"])
+  apply(rule exI[of _ "rrename \<sigma> P'"])   
   apply(cases t) unfolding ssbij_def small_def Tmap_def Vmap_def 
   by (simp add: term.rrename_comps) . . 
   (* *)
   subgoal apply(rule disjI2, rule disjI2, rule disjI1)
-  subgoal apply(elim exE) subgoal for x e e'
-  apply(rule exI[of _ "\<sigma> x"])
-  apply(rule exI[of _ "rrename_term \<sigma> e"]) apply(rule exI[of _ "rrename_term \<sigma> e'"]) 
+  subgoal apply(elim exE) subgoal for P act P' y
+  apply(rule exI[of _ "rrename \<sigma> P"])
+  apply(rule exI[of _ "map_action \<sigma> act"])
+  apply(rule exI[of _ "rrename \<sigma> P'"])
+  apply(rule exI[of _ "\<sigma> y"]) 
   apply(cases t) unfolding ssbij_def small_def Tmap_def Vmap_def 
-  by (simp add: term.rrename_comps) . . 
+  apply (simp add: term.rrename_comps) 
+  by (auto simp add: action.map_id action.map_comp) . .
   (* *)
-  subgoal apply(rule disjI2, rule disjI2, rule disjI2)
-  subgoal apply(elim exE) subgoal for x e1 e1' e2 e2'
-  apply(rule exI[of _ "\<sigma> x"])
-  apply(rule exI[of _ "rrename_term \<sigma> e1"]) apply(rule exI[of _ "rrename_term \<sigma> e1'"]) 
-  apply(rule exI[of _ "rrename_term \<sigma> e2"]) apply(rule exI[of _ "rrename_term \<sigma> e2'"]) 
+  subgoal apply(rule disjI2, rule disjI2, rule disjI2, rule disjI1)
+  subgoal apply(elim exE) subgoal for P a x P' y
+  apply(rule exI[of _ "rrename \<sigma> P"])
+  apply(rule exI[of _ "\<sigma> a"]) 
+  apply(rule exI[of _ "\<sigma> x"]) 
+  apply(rule exI[of _ "rrename \<sigma> P'"])
+  apply(rule exI[of _ "\<sigma> y"])   
   apply(cases t) unfolding ssbij_def small_def Tmap_def Vmap_def 
-  apply (simp add: term.rrename_comps) apply(subst rrename_tvsubst_comp) by auto
- . . . 
+  apply (simp add: term.rrename_comps) 
+  by auto . .
+  (* *)
+  subgoal apply(rule disjI2, rule disjI2, rule disjI2, rule disjI2, rule disjI1)
+  subgoal apply(elim exE) subgoal for P1 act P1' P2
+  apply(rule exI[of _ "rrename \<sigma> P1"])
+  apply(rule exI[of _ "map_action \<sigma> act"])
+  apply(rule exI[of _ "rrename \<sigma> P1'"])
+  apply(rule exI[of _ "rrename \<sigma> P2"])
+  apply(cases t) unfolding ssbij_def small_def Tmap_def Vmap_def 
+  apply (simp add: term.rrename_comps)  
+  by (auto simp add: action.map_id action.map_comp) . .
+  (* *)
+  subgoal apply(rule disjI2, rule disjI2, rule disjI2, rule disjI2, rule disjI2, rule disjI1)
+  subgoal apply(elim exE) subgoal for P1 a x P1' P2 P2'
+  apply(rule exI[of _ "rrename \<sigma> P1"])
+  apply(rule exI[of _ "\<sigma> a"])
+  apply(rule exI[of _ "\<sigma> x"])
+  apply(rule exI[of _ "rrename \<sigma> P1'"])
+  apply(rule exI[of _ "rrename \<sigma> P2"])
+  apply(rule exI[of _ "rrename \<sigma> P2'"])
+  apply(cases t) unfolding ssbij_def small_def Tmap_def Vmap_def 
+  by (simp add: term.rrename_comps) . .
+  (* *)
+  subgoal apply(rule disjI2, rule disjI2, rule disjI2, rule disjI2, rule disjI2, rule disjI2)
+  subgoal apply(elim exE) subgoal for P1 a x P1' P2 P2'
+  apply(rule exI[of _ "rrename \<sigma> P1"])
+  apply(rule exI[of _ "\<sigma> a"])
+  apply(rule exI[of _ "\<sigma> x"])
+  apply(rule exI[of _ "rrename \<sigma> P1'"])
+  apply(rule exI[of _ "rrename \<sigma> P2"])
+  apply(rule exI[of _ "rrename \<sigma> P2'"])
+  apply(cases t) unfolding ssbij_def small_def Tmap_def Vmap_def 
+  apply (simp add: term.rrename_comps)
+  by auto . . .
+  (* *)
+
+(* *)
+
+lemma Inp_refresh: 
+"xx \<notin> FFVars P \<or> xx = x \<Longrightarrow> Inp a x P = Inp a xx (swap P x xx)"
+sorry
+
+lemma Res_refresh: 
+"xx \<notin> FFVars P \<or> xx = x \<Longrightarrow> Res x P = Res xx (swap P x xx)"
+sorry
+
+definition "sw a x y \<equiv> if a = x then y else if a = y then x else a"
+
+lemma swap_usub: 
+"swap (usub P u x) z1 z2 = usub (swap P z1 z2) (sw u z1 z2) (sw x z1 z2)"
+sorry
+
+lemma usub_refresh: 
+"xx \<notin> FFVars P \<or> xx = x \<Longrightarrow> usub P u x = usub (swap P x xx) u xx"
+sorry
+
+(*  *)
+
+find_theorems FFVars vvsubst
   
 
 lemma fresh: "\<exists>xx. xx \<notin> Tfvars t"  
-by (metis Abs_avoid Tfvars.elims term.card_of_FFVars_bounds term.set(2))
+using Abs_avoid small_Tfvars small_def by blast 
+
+lemma fresh2: "\<exists>xx1 xx2. xx1 \<noteq> xx2 \<and> {xx1,xx2} \<inter> Tfvars t = {}"  
+using fresh[of t] apply safe subgoal for xx apply(rule exI[of _ xx])
+apply auto
+using Abs_avoid small_Tfvars small_def
+by (metis FFVars_commit_simps(1) UnCI commit_internal.card_of_FFVars_bounds(2) 
+finite_Un finite_iff_le_card_var insert_iff) .
+
+lemma fresh_n: "\<exists>xxs. length xxs = n \<and> set xxs \<inter> Tfvars t = {}"
+sorry
+
+lemma id_upd_same[simp]: "id(y := y) = id"
+  by auto
+
+fun permOfAct where 
+"permOfAct xx (bout a x) = id(x:=xx)"
+|
+"permOfAct xx _ = id"
+
+lemma bvars_act_bout: "bvars act = [] \<or> (\<exists>a b. act = bout a b)"
+by(cases act, auto)
 
 (* NB: The entities affected by variables are passed as witnesses to exI 
 with x and (the fresh) xx swapped, whereas the non-affected ones are passed 
@@ -122,53 +328,82 @@ as they are.
 lemma GG_fresh: 
 "(\<forall>\<sigma> t. ssbij \<sigma> \<and> R t \<longrightarrow> R (Tmap \<sigma> t)) \<Longrightarrow> G R v t \<Longrightarrow> 
  \<exists>w. Vfvars w  \<inter> Tfvars t = {} \<and> G R w t"
-using fresh[of t] unfolding G_def Tmap_def Vmap_def apply safe
-  subgoal for xx
-  apply(rule exI[of _ "[]"])  
+using fresh2[of t] unfolding G_def Tmap_def Vmap_def apply(elim disjE exE conjE)
+  subgoal for xx x xx1 a u P
+  apply(rule exI[of _ "[xx]"])  
   apply(rule conjI)
     subgoal unfolding ssbij_def small_def Vmap_def by auto 
-    subgoal apply(rule disjI1) by simp .
+    subgoal apply(rule disjI1) 
+    apply(rule exI[of _ "xx"]) 
+    apply(rule exI[of _ "a"])
+    apply(rule exI[of _ "u"]) 
+    apply(rule exI[of _ "swap P x xx"])
+    apply(cases t) 
+    by (simp add: Inp_refresh usub_refresh) . 
   (* *)
-  subgoal for xx e1 e1' e2 e2'
-  apply(rule exI[of _ "[]"])  
+  subgoal for xx P xx1 a x P'
+  apply(rule exI[of _ "[xx]"])  
   apply(rule conjI)
     subgoal unfolding ssbij_def small_def Vmap_def by auto 
     subgoal apply(rule disjI2, rule disjI1) 
-    apply(rule exI[of _ "e1"]) 
-    apply(rule exI[of _ "e1'"])
-    apply(rule exI[of _ "e2"]) 
-    apply(rule exI[of _ "e2'"])
-    apply(cases t)  apply simp . .
-  (* *)
-  subgoal for xx x e e'
-  apply(rule exI[of _ "[xx]"])  
-  apply(rule conjI)
-    subgoal unfolding ssbij_def small_def Vmap_def by auto 
-    subgoal apply(rule disjI2, rule disjI2, rule disjI1) 
-    apply(rule exI[of _ "xx"]) 
-    apply(rule exI[of _ "rrename_term (id(x:=xx,xx:=x)) e"])
-    apply(rule exI[of _ "rrename_term (id(x:=xx,xx:=x)) e'"])
+    apply(rule exI[of _ "swap P x xx"])
+    apply(rule exI[of _ "a"]) 
+    apply(rule exI[of _ "xx"])
+    apply(rule exI[of _ "swap P' x xx"]) 
     apply(cases t)  apply simp apply(intro conjI)
-      subgoal apply(subst Abs_rrename[of "id(x:=xx,xx:=x)"]) by auto
-      subgoal apply(subst Abs_rrename[of "id(x:=xx,xx:=x)"]) by auto
-      subgoal by (metis supp_swap_bound Prelim.bij_swap ssbij_def) . . 
+      subgoal using Res_refresh by blast
+      subgoal by auto
+      apply(erule allE[of _ "id(x:=xx,xx:=x)"])
+      apply(erule allE[of _ "P"])
+      apply(erule allE[of _ "Fout a x P'"]) 
+      by (auto simp: ssbij_def split: if_splits ) .
   (* *)
-  subgoal for xx x e1 e1' e2 e2'
-  apply(rule exI[of _ "[xx]"])  
-  apply(rule conjI)
-    subgoal unfolding ssbij_def small_def Vmap_def by auto 
-    subgoal apply(rule disjI2, rule disjI2, rule disjI2)
-    apply(rule exI[of _ "xx"]) 
-    apply(rule exI[of _ "rrename_term (id(x:=xx,xx:=x)) e1"])
-    apply(rule exI[of _ "rrename_term (id(x:=xx,xx:=x)) e1'"])
-    apply(rule exI[of _ "e2"])
-    apply(rule exI[of _ "e2'"])
-    apply(cases t)  apply simp apply(intro conjI)
-      subgoal apply(subst Abs_rrename[of "id(x:=xx,xx:=x)"]) by auto
-      subgoal apply(subst tvsubst_Var_rrename_term) 
-      apply (auto split: if_splits)   
-      by blast
-      subgoal by (metis supp_swap_bound Prelim.bij_swap ssbij_def) . . . 
+  subgoal for yy P xa act P' y 
+  using bvars_act_bout[of act] apply(elim disjE exE)
+    subgoal
+    apply(rule exI[of _ "[yy]"])  
+    apply(rule conjI)
+      subgoal unfolding ssbij_def small_def Vmap_def by auto 
+      subgoal apply(rule disjI2, rule disjI2, rule disjI1) 
+      apply(rule exI[of _ "swap P y yy"])
+      apply(rule exI[of _ "swapa act y yy"]) 
+      apply(rule exI[of _ "swap P' y yy"])
+      apply(rule exI[of _ "yy"]) 
+      apply(cases t) apply simp apply(intro conjI)
+        subgoal using Res_refresh by blast
+        subgoal using Res_refresh apply(cases act, simp_all split: if_splits)  
+          by blast+
+        subgoal by auto
+        subgoal apply(erule allE[of _ "id(y:=yy,yy:=y)"])
+        apply(erule allE[of _ "P"])
+        apply(erule allE[of _ "Cmt act P'"]) 
+        by (auto simp: ssbij_def split: if_splits ) . .
+    subgoal for a b
+    apply(rule exI[of _ "[xa,yy]"])  
+    apply(rule conjI)
+      subgoal unfolding ssbij_def small_def Vmap_def by auto 
+      subgoal apply(rule disjI2, rule disjI2, rule disjI1) 
+      apply(rule exI[of _ "swap (swap P y yy) xa a"]) 
+      apply(rule exI[of _ "swapa (swapa act y yy) xa a"]) 
+      apply(rule exI[of _ "swap (swap P' y yy) xa a"])
+      apply(rule exI[of _ "yy"]) 
+      apply(cases t) apply(intro conjI)
+        subgoal apply simp  
+        subgoal using Res_refresh by blasts
+        subgoal using Res_refresh apply(cases act, simp_all split: if_splits)  
+          by blast+
+        subgoal by auto
+        subgoal apply(erule allE[of _ "id(y:=yy,yy:=y)"])
+        apply(erule allE[of _ "P"])
+        apply(erule allE[of _ "Cmt act P'"]) 
+        by (auto simp: ssbij_def split: if_splits ) .
+      
+
+      subgoal by auto
+      apply(erule allE[of _ "id(x:=xx,xx:=x)"])
+      apply(erule allE[of _ "P"])
+      apply(erule allE[of _ "Fout a x P'"]) 
+      by (auto simp: ssbij_def split: if_splits) .  
   (* *)
 
 
